symbolic_execution.v
@@ -1,36 +1,37 @@
+Require Import Ensembles. 
+
 Module ConcState.
-(*Variable conc_state : Type.*)
 
-Inductive conc_state : Type :=
-|concstate
-|NextState (x: conc_state).
-
-Inductive conc_state_set : Type :=
-|Empty 
-|Cons (x : conc_state) (s: conc_state_set).
+Variable input : Type.
 
 
+Inductive input_list : Type :=
+|EmptyList
+|ConsList (i : input) (s : input_list).
 
-(*Definition conc_state_set := conc_state -> Prop.*)
+Fixpoint in_input_list (l : input_list) (i : input) : Prop :=
+match l with
+|EmptyList => False
+|ConsList item i_list => (item = i) \/ (in_input_list i_list i)
+end . 
 
-Fixpoint In (A:conc_state_set) (x:conc_state) : Prop := 
-match A with 
-|Empty => False
-|Cons y s => (y=x) \/ In s x
-end.
 
-(*Definition Included (B C:conc_state_set) : Prop := forall x:conc_state, In B x -> In C x.
+(*Inductive conc_state : Type :=
+|concstate.*)
 
-Inductive Empty_set : conc_state_set :=.*)
+
+Variable conc_state : Type.
 
 
 (* conc_ex(A) returns ConcState that results from 
 the concrete execution of ConcState A  *)
+Definition concrete_execution := Ensemble conc_state -> input -> Ensemble conc_state.
+
+Axiom conc_ex : concrete_execution.
 
 
-
-
-
+Definition singleton (l : conc_state) : Ensemble conc_state :=
+  Add conc_state (Empty_set conc_state) l.
 
 
 
@@ -42,28 +43,17 @@ Import ConcState.
 
 
 
-
-
-
-
 Module System.
 (* System initializes with a defined set of
  initial configuration states, InitStates *)
-(*Inductive init_conc_states : Set :=
-| IsConc (a : ConcState.conc_state).*)
 
 
-Definition conc_ex (A: ConcState.conc_state) : ConcState.conc_state := 
-match A with
-|concstate => NextState A
-|NextState x => NextState (NextState x)
-end.
 
-Fixpoint conc_ex_n (x: ConcState.conc_state) (n:nat) : ConcState.conc_state :=
+(*Fixpoint conc_ex_n (x: ConcState.conc_state) (n:nat) : ConcState.Ensemble conc_state :=
 match n with
-|0 => x
+|0 => Cons x Empty
 |S n' => conc_ex (conc_ex_n x (n'))
-end.
+end.*)
 
 End System.
 
@@ -71,116 +61,106 @@ Import System.
 
 Module SymbolicExec.
 
-Variable Phi PC : Type.
-
-
-
-
-(*Variable general_set : conc_state_set.*)
-
-(*Definition unif (x : SymbolicExec.sym_state) : conc_state_set := general_set.*)
-
-(* sym_ex(A) returns an object
- in the equivalence class of SymbolicExec
- that results from 
-the symbolic execution of an object
-in the equivalence class of SymbolicExec A  *)
-
-
-(*Inductive sym_state : Type :=
-|ConstructState (a : Phi) (p : PC)
-|SymEx (x : sym_state)
-|Intermediate_Sym_Ex (x : sym_state).*)
 
 (* Symbolic state contains abstract state 
 and path constraint. *)
+
+
+Variable Phi PC : Type.
+
 Inductive sym_state: Type :=
 |ConstructState (a : Phi) (p : PC)
-|SymEx (x : sym_state).
+|nilstate.
 
 
-Definition up_pc := PC -> PC.
-Axiom update_pc : up_pc.
-Definition up_phi := Phi -> Phi.
-Axiom update_phi: up_phi.
+
+Definition up_pc_l := PC -> PC.
+Axiom update_pc_left : up_pc_l.
+
+Definition up_pc_r := PC -> PC.
+Axiom update_pc_right : up_pc_r.
+
+Definition up_phi_l := Phi -> Phi.
+Axiom update_phi_left: up_phi_l.
+
+Definition up_phi_r := Phi -> Phi.
+Axiom update_phi_right: up_phi_r.
 
 (* get_phi returns abstract state *)
-Fixpoint get_phi (x : sym_state) : Phi :=
-match x with
-|ConstructState phi pc => phi
-|SymEx a => update_phi (get_phi a)
-end.
+Definition get_sym_state  :=  sym_state -> Phi.
+Axiom get_phi : get_sym_state.
 
 (* get_pc returns the path constraint *)
-Fixpoint get_pc (x : sym_state) : PC :=
-match x with
-|ConstructState phi pc => pc
-|SymEx a => update_pc (get_pc a)
-end.
+Definition get_path_constraint := sym_state -> PC.
+Axiom get_pc : get_path_constraint.
 
-Fixpoint sym_ex (A:sym_state) : sym_state:=
-match A with 
-| ConstructState phi pc => SymEx A
-| SymEx a => SymEx (sym_ex a)
-end.
+(*Definition sym_execution := sym_state -> sym_state.
+Axiom sym_ex : sym_execution.*)
 
-
-(*Class SymExec (pc phi: Type) := {
-  get_phi : phi -> Phi ;
-  get_pc : pc -> PC;
-  update_phi : phi -> Prop;
-  update_pc : pc -> Prop;
-  cons_state : pc -> phi -> sym_state;
-  unif : pc -> phi -> conc_state_set;
-  sym_ex : pc -> phi -> sym_state;
-  intermediate_sym_ex : phi -> sym_state}.*)
-
-
-Fixpoint sym_ex_n (x:sym_state) (n:nat) : sym_state :=
+(*Fixpoint sym_ex_n (x:sym_state) (n:nat) : sym_state :=
 match n with
 |0 => x
 |S n' => sym_ex (sym_ex_n x (n'))
 end.
+*)
 
+Definition uni := Phi -> PC -> Ensemble ConcState.conc_state.
 
-(* unif(A) returns the set of concrete states
- represented by symbolic state A. *)
-(* Not convinced that this is saying what I want it to. 
-I think it's returning the entire set of conc states, not just a subset.*)
-(*Definition unif (A:sym_state) : ConcState.conc_state_set :=
-match A with 
-| sym_state => ConcState.conc_state_set
-end.*)
-
-Definition uni := sym_state -> ConcState.conc_state_set.
 Axiom unif : uni.
 
-(* is_leaf(T, n) returns true if
- n is a leaf in tree T. *)
-(* is_root(T, n) returns true if
- n is a root in tree T. *)
-(* get_root(T) returns the root of tree T. *)
-(*Modified version of FSet RBT https://github.com/coq-contribs/fsets/blob/master/FSetRBT.v *)
-Definition state := SymbolicExec.sym_state.
+
 
 Inductive SE_tree : Type :=
 | leaf: SE_tree
-| sym_node: SE_tree -> state -> SE_tree -> SE_tree
-| intermediate_node : SE_tree -> state ->SE_tree.
+| ConsNode: SE_tree -> sym_state -> SE_tree -> SE_tree.
 
-Fixpoint max (m n : nat) : nat :=
-match m, n with
-|0, _ => n
-|S m', 0 => m
-|S m', S n' => S (max m' n')
+Definition root (t : SE_tree) : sym_state :=
+match t with 
+|leaf => nilstate
+|ConsNode l n r => n
 end.
 
-Fixpoint tree_height (t : SE_tree) : nat :=
+(*Fixpoint tree_height (t : SE_tree) : nat :=
 match t with
 |leaf => O
-|sym_node l n r  => S (max (tree_height l) (tree_height r))
-|intermediate_node child n => S (tree_height child)
+|ConsNode l n r  => S (max (tree_height l) (tree_height r))
 end.
+*)
+
+Fixpoint is_leaf_state (tree : SE_tree) (state : sym_state) : Prop :=
+match tree with 
+|leaf => False
+|ConsNode l n r => 
+  ((n = state) /\ (l = leaf))
+  \/ (is_leaf_state l state)
+  \/ (is_leaf_state r state)
+end.
+
+Definition left_child (tree : SE_tree) : sym_state :=
+match tree with 
+|leaf => nilstate
+|ConsNode l n r => root l
+end.
+
+Definition right_child (tree : SE_tree) : sym_state :=
+match tree with 
+|leaf => nilstate
+|ConsNode l n r => root r
+end.
+
+
+Definition sym_ex_with_branching (state : sym_state) : SE_tree :=
+match state with 
+|ConstructState phi pc => 
+ConsNode 
+(ConsNode leaf (ConstructState (update_phi_left phi ) (update_pc_left pc)) leaf)
+ state
+(ConsNode leaf (ConstructState (update_phi_right phi ) (update_pc_right pc)) leaf)
+|nilstate => leaf
+end.
+
+
+
 
 Inductive SE_tree_list : Type :=
 |nil: SE_tree_list
@@ -197,47 +177,124 @@ Fixpoint length (l:SE_tree_list) : nat :=
   end.
 
 
-Fixpoint in_tree_list  (tlist : SE_tree_list) (x : SymbolicExec.SE_tree) : Prop :=
+
+
+Fixpoint in_tree_list  (tlist : SE_tree_list) (x : SE_tree) : Prop :=
 match tlist with 
 |nil => False
 |h :: t => (x = h) \/ (in_tree_list t x)
 end.
 
+Definition head (tlist : SE_tree_list) : SE_tree :=
+match tlist with 
+|nil => leaf
+|h :: t => h
+end.
+
+Definition second_elem (tlist : SE_tree_list) : SE_tree :=
+match tlist with
+|nil => leaf
+|h :: t => (head t)
+end.
+
+Fixpoint tail (tlist : SE_tree_list) : SE_tree :=
+match tlist with 
+|nil => leaf
+|h :: t => 
+  match t with
+  |nil => h
+  |tailh :: tailt => tail t
+  end
+end.
+
+(*is_consecutive_in_order checks if A and B are consecutive in the tree list
+and if A comes before B *)
+Fixpoint is_consecutive_in_order (A B : SE_tree) (tlist : SE_tree_list) : Prop :=
+match tlist with 
+|nil => False
+|h :: t => 
+  ((A = h) /\  (B = (head t))) 
+  \/ (is_consecutive_in_order A B t)
+end.
 
 
 
-Definition is_leaf (T: SE_tree) (n : SymbolicExec.sym_state) : Prop := True.
+Definition is_connected  (tlist : SE_tree_list) : Prop :=
+ forall (A B : SE_tree), 
+ (is_consecutive_in_order A B tlist) ->
+  is_leaf_state A (root B). 
+
+Inductive Sym_state_list : Type :=
+|nil_list: Sym_state_list
+|sscons: sym_state -> Sym_state_list -> Sym_state_list.
+
+(*Notation "x :: l" := (sscons x l) (at level 60, right associativity).
+Notation "[ ]" := endstate.
+Notation "[ x ; .. ; y ]" := (sscons x .. (sscons y nil) ..).*)
+
+
+(*Fixpoint list_of_leaf_states (tlist : SE_tree_list) : Sym_state_list:=
+match tlist with
+|nil => nil_list
+|h :: t => 
+  match t with 
+    |nil => nil_list
+    |headt :: tailt => sscons (root (head t)) (list_of_leaf_states t)
+  end
+end.
+
+Fixpoint remove_tail (slist : Sym_state_list) : Sym_state_list :=
+match slist with 
+|nil_list => nil_list
+|sscons h t => 
+  match t with
+  |nil_list => nil_list
+  |sscons headt tailt => sscons h (remove_tail t) 
+  end
+end.*)
+
+(*Fixpoint state_list_execution (slist : Sym_state_list) : Ensemble conc_state :=
+match slist with
+|nil_list => Empty 
+|sscons h t => 
+  match t with 
+  |nil_list => conc_ex (unif h)
+  |sscons headt tailt => conc_ex (state_list_execution (remove_tail slist))
+  end
+end.*)
 
 
 
+
+(*
 (* SE Properties Go Here *)
 Axiom lem_1 : forall (conc1 conc2 : ConcState.conc_state)
  (sym1: SymbolicExec.sym_state),
-(conc_ex conc1 = conc2) /\ (In (unif sym1) conc1)  ->
+(conc_ex (singleton conc1) = (singleton conc2)) /\ (In (unif (get_phi sym1) (get_pc sym1)) conc1)  ->
 exists sym2, 
-(In (unif sym2) conc2) /\ sym_ex sym1 = sym2. 
+(In (unif (get_phi sym2) (get_pc sym2)) conc2) /\ sym_ex sym1 = sym2. 
 
 Axiom lem_1_n : forall (conc1 conc2 : ConcState.conc_state)
  (sym1: SymbolicExec.sym_state) (n : nat),
-(conc_ex_n conc1 n = conc2) /\ (In (unif sym1) conc1)  ->
+(conc_ex_n conc1 n = (Cons conc2 Empty)) /\ (In (unif (get_phi sym1) (get_pc sym1)) conc1)  ->
 exists sym2, 
-(In (unif sym2) conc2) /\ sym_ex_n sym1 n = sym2.
+(In (unif (get_phi sym2) (get_pc sym2)) conc2) /\ sym_ex_n sym1 n = sym2.
 
 Axiom lem_2 : forall (conc2 : ConcState.conc_state)
  (sym1 sym2: SymbolicExec.sym_state),
-(sym_ex sym1 = sym2) /\ (In (unif sym2) conc2)  ->
+(sym_ex sym1 = sym2) /\ (In (unif (get_phi sym2) (get_pc sym2)) conc2)  ->
 exists conc1, 
-(In (unif sym1) conc1) /\ 
-(conc_ex conc1 = conc2).
+(In (unif (get_phi sym1) (get_pc sym1)) conc1) /\ 
+((conc_ex (Cons conc1 Empty)) = (Cons conc2 Empty)).
 
 Axiom lem_2_n : forall (conc2 : ConcState.conc_state)
  (sym1 sym2: SymbolicExec.sym_state) (n:nat),
-(sym_ex_n sym1 n = sym2) /\ (In (unif sym2) conc2)  ->
+(sym_ex_n sym1 n = sym2) /\ (In (unif (get_phi sym2) (get_pc sym2)) conc2)  ->
 exists conc1, 
-(In (unif sym1) conc1) /\ 
-(conc_ex_n conc1 n = conc2).
+(In (unif (get_phi sym1) (get_pc sym1)) conc1) /\ 
+(conc_ex_n conc1 n = (Cons conc2 Empty)).
 
-
+*)
 
 
 
@@ -250,48 +307,51 @@ End SymbolicExec.
 Import SymbolicExec. 
 
 
-Module SymbolicExecList. 
-
-
-
-End SymbolicExecList.
-
-Import SymbolicExecList.
 
 Module SERecurs.
 
+(* Takes as input symbolic state of root and pc of its leaf 
+and returns all and only the concrete states that will take us down 
+the path that leads to the leaf. *)
+Definition circle_op_1 (sym sym_leaf : SymbolicExec.sym_state) : Ensemble ConcState.conc_state :=
+unif (get_phi sym) (get_pc sym_leaf).
 
-Definition circle_op_1 (sym : SymbolicExec.sym_state) : ConcState.conc_state_set :=
-unif sym.
+(*Takes as input symbolic state of leaf state and pc of leaf state 
+and returns concrete states that correspond *)
+Definition circle_op_2 (sym : SymbolicExec.sym_state) : Ensemble ConcState.conc_state :=
+unif (get_phi sym) (get_pc sym).
 
-Definition circle_op_2 (sym : SymbolicExec.sym_state) : ConcState.conc_state_set :=
-unif (sym_ex sym).
 
-Fixpoint set_in_set (set1 set2 : ConcState.conc_state_set) : Prop :=
-match set1 with 
-|Empty => (set2 = Empty) \/ False
-|Cons y s => (set1 = set2) \/ (set_in_set s set2)
-end.
 
-Variable init_conc_states: ConcState.conc_state_set.
 
-(* 3 properties and sufficiency go here *)
-Variable ErrorStates: ConcState.conc_state_set.
+
+
+Variable init_conc_states: Ensemble ConcState.conc_state.
+
+
+Variable ErrorStates: Ensemble ConcState.conc_state.
 
 Variable tree_list : SymbolicExec.SE_tree_list.
-(* NEED TREE LIST GENERATION *)
 
 
-Definition is_connected (tlist : SymbolicExec.SE_tree_list) : Prop := True.
 
 
-Axiom properties : forall (e : SymbolicExec.SE_tree), 
-in_tree_list tree_list e -> 
-exists n,
-(SymbolicExec.is_leaf e n)
-/\(set_in_set init_conc_states  (circle_op_1 n))
-/\ (set_in_set  ErrorStates (circle_op_2 n))
+
+
+Axiom properties : 
+(Included ConcState.conc_state 
+init_conc_states
+(circle_op_1 (root(head tree_list)) (root (second_elem tree_list))))
+/\ (((Intersection ConcState.conc_state  ErrorStates (circle_op_2 (right_child (tail tree_list))) 
+<> Empty_set ConcState.conc_state))
+\/((Intersection ConcState.conc_state  ErrorStates (circle_op_2 (left_child (tail tree_list))) 
+<> Empty_set ConcState.conc_state)))
 /\ (is_connected tree_list). 
+
+
+(*
+Theorem sufficiency : forall (tree : SE_tree), 
+tree*)
 
 End SERecurs.
 
